length of argvals/retvals is already checked in semantics,
so phase composition does not need to treat it specially.
Also make sure that locals_based_call_spec enforces that argvals
matches length of argnames.

compiler/src/compiler/MMIO.v
@@ -119,7 +119,7 @@ Section MMIO1.
        morphism (word.ring_morph (word := word)),
        constants [word_cst]).
 
-  Definition compile_ext_call(_: funname_env (nat * nat * Z))(_ _: Z)(s: stmt Z) :=
+  Definition compile_ext_call(_: funname_env Z)(_ _: Z)(s: stmt Z) :=
       match s with
       | SInteract resvars action argvars => compile_interact resvars action argvars
       | _ => []
@@ -374,7 +374,7 @@ Section MMIO1.
       split; eauto.
       split; eauto.
       split; eauto.
-      split; eauto. 
+      split; eauto.
       split. {
         lazymatch goal with
         | H: map.undef_on initialL_mem ?A |- _ =>
